replace at_addr by sepcl, which also takes a value,
so that use sites of sepcl can remain unchanged if we want
to swap addr/value order of all sep predicates, and we
don't need two versions of each predicate any more
(deleting SepAddrLast.v).
Moreover, sepcl enables notations that want to identify
not only "the address", but also "the value" and "the
predicate" of a clause.

bedrock2/src/bedrock2/SepAutoArray.v
@@ -7,18 +7,18 @@ Require Import coqutil.Word.Bitwidth.
 Require Import coqutil.Tactics.rewr.
 
 Definition with_len{width}{word: word width}{mem: map.map word byte}{V: Type}
-  (n: nat)(array_pred: list V -> word -> mem -> Prop)(vs: list V)(a: word): mem -> Prop :=
-  with_pure (a |-> array_pred vs) (List.length vs = n).
+  (n: nat)(array_pred: sep_predicate mem (list V)): sep_predicate mem (list V) :=
+  fun (a: word) (vs: list V) => with_pure (sepcl array_pred vs a) (List.length vs = n).
 
 Section SepLog.
   Context {width: Z} {BW: Bitwidth width} {word: word.word width} {mem: map.map word byte}.
   Context {word_ok: word.ok word} {mem_ok: map.ok mem}.
 
-  Lemma with_len_eq[V: Type]: forall (array_pred: list V -> word -> mem -> Prop) vs n,
+  Lemma with_len_eq[V: Type]: forall (array_pred: sep_predicate mem (list V)) vs n,
       List.length vs = n ->
-      with_len n array_pred vs = array_pred vs.
+      sepcl (with_len n array_pred) vs = sepcl array_pred vs.
   Proof.
-    intros. unfold with_len, with_pure, at_addr. extensionality a.
+    intros. unfold with_len, with_pure, sepcl. extensionality a.
     replace (List.length vs = n) with True.
     - eapply iff1ToEq. cancel.
     - apply propositional_extensionality. split; auto.
@@ -31,31 +31,20 @@ Section SepLog.
   Qed.
 
   Lemma extract_with_len[V: Type]:
-    forall [array_pred: list V -> word -> mem -> Prop] [vs n m R a],
-      sep (a |-> with_len n array_pred vs) R m -> List.length vs = n.
+    forall [array_pred: sep_predicate mem (list V)] [vs n m R a],
+      sep (a :-> vs : with_len n array_pred) R m -> List.length vs = n.
   Proof.
     intros. eapply extract_pure in H. exact H.
   Qed.
 
-  (* There's some tradeoff in the choice whether sz should be a Z or a word:
-     If it's a Z, lemmas need an explicit sidecondition to upper-bound it,
-     which we get for free if it's a word, but then we need to convert it
-     back to Z in many places, so when lemmas are used with sz := (word.of_Z n),
-     we'll have to rewrite many occurrences of (word.unsigned (word.of_Z n))
-     into n, which seems more expensive than simply proving the sidecondition. *)
-
-  Definition array{E: Type}(elem: E -> word -> mem -> Prop)(sz: Z)(vs: list E)
-             (addr: word): mem -> Prop :=
-    bedrock2.Array.array (fun a e => elem e a) (word.of_Z sz) addr vs.
-
-  Lemma array_app{E : Type}{elem: E -> word ->  mem -> Prop}{sz: Z}:
+  Lemma array_app{E : Type}{elem: sep_predicate mem E}{sz: Z}:
     forall (xs ys: list E) (start : word),
-      (start |-> array elem sz (xs ++ ys)) =
-      (sep (start |-> array elem sz xs)
-           (word.add start (word.of_Z (sz * Z.of_nat (Datatypes.length xs))) |->
-               array elem sz ys)).
+      (start :-> xs ++ ys : array elem (word.of_Z sz)) =
+      (sep (start :-> xs : array elem (word.of_Z sz))
+           (word.add start (word.of_Z (sz * Z.of_nat (Datatypes.length xs))) :-> ys
+             : array elem (word.of_Z sz))).
   Proof.
-    unfold array, at_addr.
+    unfold sepcl.
     intros.
     eapply iff1ToEq.
     etransitivity.
@@ -68,24 +57,25 @@ Section SepLog.
     reflexivity.
   Qed.
 
-  Lemma access_elem_in_array: forall a a' E (elem: E -> word -> mem -> Prop) vsOld vOld sz,
+  Lemma access_elem_in_array: forall a a' E (elem: sep_predicate mem E) vsOld vOld sz,
       0 < sz < 2 ^ width ->
       word.unsigned (word.sub a' a) mod sz = 0 ->
       let i := Z.to_nat (word.unsigned (word.sub a' a) / sz) in
       (* only here to make sure automation picks the right array *)
       (i < List.length vsOld)%nat ->
-      split_sepclause (a |-> array elem sz vsOld) (a' |-> elem vOld)
+      split_sepclause (a :-> vsOld : array elem (word.of_Z sz)) (a' :-> vOld : elem)
         (forall vs vs1 v vs2,
            (* connected with /\ because it needs to be solved by considering both at once *)
            vs = vs1 ++ [v] ++ vs2 /\ List.length vs1 = i ->
            iff1 (seps
-              [a |-> array elem sz vs1;
-               a' |-> elem v;
-               word.add a (word.of_Z (sz * Z.of_nat (S i))) |-> array elem sz vs2])
-            (a |-> array elem sz vs)).
+              [a :-> vs1 : array elem (word.of_Z sz);
+               a' :-> v : elem;
+               word.add a (word.of_Z (sz * Z.of_nat (S i))) :-> vs2
+                 : array elem (word.of_Z sz)])
+            (a :-> vs : array elem (word.of_Z sz))).
   Proof.
     unfold split_sepclause.
-    unfold array, at_addr, seps.
+    unfold sepcl, seps.
     intros. fwd.
     cbn [List.app].
     symmetry.
@@ -103,21 +93,21 @@ Section SepLog.
     reflexivity.
   Qed.
 
-  Lemma access_subarray_stmt: forall a a' E (elem: E -> word -> mem -> Prop) sz n,
+  Lemma access_subarray_stmt: forall a a' E (elem: sep_predicate mem E) sz n,
       0 < sz < 2 ^ width ->
       word.unsigned (word.sub a' a) mod sz = 0 ->
       let i := Z.to_nat (word.unsigned (word.sub a' a) / sz) in
       (forall vs vs1 vs2 vs3,
           vs = vs1 ++ vs2 ++ vs3 /\ List.length vs1 = i /\ List.length vs2 = n ->
            iff1 (seps
-              [a |-> array elem sz vs1;
-               a' |-> array elem sz vs2;
-               word.add a (word.of_Z (sz * Z.of_nat (i + n))) |->
-                        array elem sz vs3])
-            (a |-> array elem sz vs)).
+              [a :-> vs1 : array elem (word.of_Z sz);
+               a' :-> vs2 : array elem (word.of_Z sz);
+               word.add a (word.of_Z (sz * Z.of_nat (i + n))) :-> vs3
+                 : array elem (word.of_Z sz)])
+            (a :-> vs : array elem (word.of_Z sz))).
   Proof.
     intros.
-    unfold array, at_addr, seps.
+    unfold sepcl, seps.
     intros. fwd.
     symmetry.
     rewrite 2array_append.
@@ -133,89 +123,90 @@ Section SepLog.
   Qed.
 
   (* used when the length of vsPart can be computed with concrete_length *)
-  Lemma access_subarray_concrete_length: forall a a' E (elem: E -> word -> mem -> Prop) sz n
+  Lemma access_subarray_concrete_length: forall a a' E (elem: sep_predicate mem E) sz n
                                                 vsAll vsPart,
       0 < sz < 2 ^ width ->
       word.unsigned (word.sub a' a) mod sz = 0 ->
       let i := Z.to_nat (word.unsigned (word.sub a' a) / sz) in
       (* only here to make sure automation picks the right array *)
       (i + n <= List.length vsAll)%nat ->
-      split_sepclause (a |-> array elem sz vsAll)
-                      (a' |-> array elem sz vsPart)
+      split_sepclause (a :-> vsAll : array elem (word.of_Z sz))
+                      (a' :-> vsPart : array elem (word.of_Z sz))
         (forall vs vs1 vs2 vs3,
            vs = vs1 ++ vs2 ++ vs3 /\ List.length vs1 = i /\ List.length vs2 = n ->
            iff1 (seps
-              [a |-> array elem sz vs1;
-               a' |-> array elem sz vs2;
-               word.add a (word.of_Z (sz * Z.of_nat (i + n))) |->
-                        array elem sz vs3])
-            (a |-> array elem sz vs)).
+              [a :-> vs1 : array elem (word.of_Z sz);
+               a' :-> vs2 : array elem (word.of_Z sz);
+               word.add a (word.of_Z (sz * Z.of_nat (i + n))) :-> vs3
+                 : array elem (word.of_Z sz)])
+            (a :-> vs : array elem (word.of_Z sz))).
   Proof.
     intros. unfold split_sepclause. intros. eapply access_subarray_stmt; eassumption.
   Qed.
 
-  Lemma access_subarray_with_len: forall a a' E (elem: E -> word -> mem -> Prop) sz n
+  Lemma access_subarray_with_len: forall a a' E (elem: sep_predicate mem E) sz n
                                          vsAll vsPart,
       0 < sz < 2 ^ width ->
       word.unsigned (word.sub a' a) mod sz = 0 ->
       let i := Z.to_nat (word.unsigned (word.sub a' a) / sz) in
       (* only here to make sure automation picks the right array *)
       (i + n <= List.length vsAll)%nat ->
-      split_sepclause (a |-> array elem sz vsAll)
-                      (a' |-> with_len n (array elem sz) vsPart)
+      split_sepclause (a :-> vsAll : array elem (word.of_Z sz))
+                      (a' :-> vsPart : with_len n (array elem (word.of_Z sz)))
         (forall vs vs1 vs2 vs3,
            vs = vs1 ++ vs2 ++ vs3 /\ List.length vs1 = i /\ List.length vs2 = n ->
            iff1 (seps
-              [a |-> array elem sz vs1;
-               a' |-> with_len n (array elem sz) vs2;
-               word.add a (word.of_Z (sz * Z.of_nat (i + n))) |->
-                        array elem sz vs3])
-            (a |-> array elem sz vs)).
+              [a :-> vs1 : array elem (word.of_Z sz);
+               a' :-> vs2 : with_len n (array elem (word.of_Z sz));
+               word.add a (word.of_Z (sz * Z.of_nat (i + n))) :-> vs3
+                 : array elem (word.of_Z sz)])
+            (a :-> vs : array elem (word.of_Z sz))).
   Proof.
     intros. unfold split_sepclause. intros.
-    unfold with_len, with_pure, at_addr. fwd.
+    unfold with_len, with_pure, sepcl. fwd.
     replace (length vs2 = length vs2) with True. 2: {
       eapply PropExtensionality.propositional_extensionality. split; auto.
     }
     etransitivity.
     2: eapply access_subarray_stmt; eauto.
-    unfold at_addr.
+    unfold sepcl.
     cbn [seps]. ecancel.
   Qed.
 
-  Lemma access_suffix: forall a a' E (elem: E -> word -> _ -> Prop) sz vsPrefix vsSuffix,
+  Lemma access_suffix: forall a a' E (elem: sep_predicate mem E) sz vsPrefix vsSuffix,
       0 < sz < 2 ^ width ->
       word.sub a' a = word.mul (word.of_Z sz)
                                (word.of_Z (Z.of_nat (List.length vsPrefix))) ->
-      split_sepclause (a |-> array elem sz (List.app vsPrefix vsSuffix))
-                      (a' |-> array elem sz vsSuffix)
+      split_sepclause (a :-> List.app vsPrefix vsSuffix : array elem (word.of_Z sz))
+                      (a' :-> vsSuffix : array elem (word.of_Z sz))
         (forall vs vs1 vs2,
            vs = vs1 ++ vs2 /\
            List.length vs1 = List.length vsPrefix /\
            List.length vs2 = List.length vsSuffix ->
-           iff1 (seps [a |-> array elem sz vs1; a' |-> array elem sz vs2])
-                (a |-> array elem sz vs)).
+           iff1 (seps [a :-> vs1 : array elem (word.of_Z sz);
+                       a' :-> vs2 : array elem (word.of_Z sz)])
+                (a :-> vs : array elem (word.of_Z sz))).
   Proof.
     intros. unfold split_sepclause. intros. fwd.
     rewrite array_app. cbn [seps].
     cancel. cbn [seps].
     match goal with
-    | |- iff1 _ (?x |-> _) => replace x with a'
+    | |- iff1 _ (?x :-> _ : _) => replace x with a'
     end.
     1: reflexivity.
     destruct width_cases; ZnWords.
   Qed.
 
-  Lemma access_tail: forall a a' E (elem: E -> word -> _ -> Prop) sz vH vsTail,
+  Lemma access_tail: forall a a' E (elem: sep_predicate mem E) sz vH vsTail,
       0 < sz < 2 ^ width ->
       word.sub a' a = word.of_Z sz ->
-      split_sepclause (a |-> array elem sz (List.cons vH vsTail))
-                      (a' |-> array elem sz vsTail)
+      split_sepclause (a :-> List.cons vH vsTail : array elem (word.of_Z sz))
+                      (a' :-> vsTail : array elem (word.of_Z sz))
         (forall v vs,
-           iff1 (seps [a |-> elem v; a' |-> array elem sz vs])
-                (a |-> array elem sz (List.cons v vs))).
+           iff1 (seps [a :-> v : elem; a' :-> vs : array elem (word.of_Z sz)])
+                (a :-> List.cons v vs : array elem (word.of_Z sz))).
   Proof.
-    intros. unfold split_sepclause. intros. unfold at_addr, array. cbn.
+    intros. unfold split_sepclause. intros. unfold sepcl. cbn.
     cancel. cbn [seps].
     match goal with
     | |- iff1 _ (Array.array _ _ ?x _) => replace x with a'
@@ -318,7 +309,7 @@ Section WithA.
   Qed.
 End WithA.
 
-Notation word_array := (array scalar 4).
+Notation word_array := (array Scalars.scalar (word.of_Z 4)).
 
 Ltac concrete_sz_bounds :=
   lazymatch goal with
@@ -336,31 +327,32 @@ Ltac concrete_sz_bounds :=
 
 (* split_sepclause_goal: *)
 
-#[export] Hint Extern 1 (split_sepclause (_ |-> array ?elem ?sz _) (_ |-> ?elem _) _) =>
+#[export] Hint Extern 1 (split_sepclause (_ :-> _ : array ?elem ?sz) (_ :-> _ : ?elem) _) =>
   eapply access_elem_in_array; [ concrete_sz_bounds | listZnWords | listZnWords ]
 : split_sepclause_goal.
 
 #[export] Hint Extern 1
-  (split_sepclause (?a |-> array ?elem ?sz ?vsAll)
-                   (?a' |-> with_len ?n (array ?elem ?sz) ?vsPart) _) =>
-  eapply (access_subarray_with_len a a' _ elem sz n vsAll vsPart);
+  (split_sepclause (?a :-> ?vsAll : array ?elem ?sz)
+                   (?a' :-> ?vsPart : with_len ?n (array ?elem ?sz)) _) =>
+  eapply (access_subarray_with_len a a' _ elem _ n vsAll vsPart);
   [ concrete_sz_bounds | listZnWords | listZnWords ]
 : split_sepclause_goal.
 
 #[export] Hint Extern 1
-  (split_sepclause (?a |-> array ?elem ?sz ?vsAll) (?a' |-> array ?elem ?sz ?vsPart) _) =>
+  (split_sepclause (?a :-> ?vsAll : array ?elem ?sz)
+                   (?a' :-> ?vsPart : array ?elem ?sz) _) =>
   let n := concrete_list_length vsPart in
-  eapply (access_subarray_concrete_length a a' _ elem sz n vsAll vsPart);
+  eapply (access_subarray_concrete_length a a' _ elem _ n vsAll vsPart);
   [ concrete_sz_bounds | listZnWords | listZnWords ]
 : split_sepclause_goal.
 
-#[export] Hint Extern 1 (split_sepclause (_ |-> array ?elem ?sz (?vs1 ++ ?vs2))
-                                         (_ |-> array ?elem ?sz ?vs2) _) =>
+#[export] Hint Extern 1 (split_sepclause (_ :-> ?vs1 ++ ?vs2 : array ?elem ?sz)
+                                         (_ :-> ?vs2 : array ?elem ?sz) _) =>
   eapply access_suffix; [ concrete_sz_bounds | listZnWords ]
 : split_sepclause_goal.
 
-#[export] Hint Extern 1 (split_sepclause (_ |-> array ?elem ?sz (_ :: ?vsTail))
-                                         (_ |-> array ?elem ?sz ?vsTail) _) =>
+#[export] Hint Extern 1 (split_sepclause (_ :-> (_ :: ?vsTail) : array ?elem ?sz)
+                                         (_ :-> ?vsTail : array ?elem ?sz) _) =>
   eapply access_tail; [ concrete_sz_bounds | listZnWords ]
 : split_sepclause_goal.
 
