bedrock2/src/bedrock2/SepClause.v
@@ -1,0 +1,27 @@
+Require Export Coq.ZArith.ZArith.
+Require Export coqutil.Byte.
+Require Export coqutil.Map.Interface coqutil.Map.Properties coqutil.Map.OfListWord.
+Require Export coqutil.Word.Interface coqutil.Word.Properties.
+Require Export bedrock2.Map.Separation bedrock2.Map.SeparationLogic.
+
+(* Try to treat this type as abstractly as possible, as we might change the
+   argument order from `word -> V -> mem -> Prop` to `V -> word -> mem -> Prop`,
+   or make it a record or typeclass with additional size info. *)
+Definition sep_predicate{width: Z}{word: word width}(mem: map.map word byte)(V: Type) :=
+  word -> V -> mem -> Prop.
+
+(* One level of indirection to:
+   - enable notations that need to detect "the address", "the value", and
+     the sep_predicate of a clause
+   - potentially infer the sep_predicate from the value type
+   - detection of "the address" of a predicate for preserving the order of clauses *)
+Definition sepcl{width: Z}{word: word width}{mem: map.map word byte}{V: Type}
+           (p: sep_predicate mem V)(v: V)(a: word): mem -> Prop := p a v.
+
+(* Precedence: `*` is at level 40, and we want to bind stronger than `*`, and moreover,
+   `^` is at level 30, and for consistency, we also want to bind stronger than `^`,
+   so we choose 25. To avoid conflict with type annotation, we put v at level 99.
+   Order: Mimics hypothesis with a body, eg in `x := 1 : Z`, the order is
+   "label, value, type". *)
+Notation "a :-> v : p" := (sepcl p v a)
+  (at level 25, v at level 99, format "a  :->  v  :  p").
